<section xml:id="polynomial-long-division">
    <title>The Division Algorithm</title>
    <subsection xml:id="division-algorithm">
  <title>Natural Numbers Version</title>

  <theorem xml:id="division-algorithm-natural-numbers">
    <title>The Division Algorithm for Natural Numbers</title>
    <statement>
      <p>Let <m>p</m> and <m>d</m> be natural numbers (nonzero, positive, whole numbers). Then there exist two unique numbers, a <term>quotient</term> <m>q</m> and a <term>remainder</term> <m>r</m>, such that <me>p = q\cdot d + r</me>, where <m>r &lt; d</m>.
    <ul>
        <li>
            <p>
                <m>p</m> is known as the <term>dividend</term>.
            </p>
        </li>
        <li>
            <p>
                <m>d</m> is known as the <term>divisor</term>.
            </p>
        </li>
    </ul></p>
    </statement>
  </theorem>

  <p>The Division Algorithm gives us a way to define division in terms of multiplication and addition for any two numbers <m>p</m> and <m>d</m>. We find the values <m>q</m> and <m>r</m> using <term>long division</term>. Our next two examples show us what happens.</p>
  <example xml:id="long-division-nonzero-remainder">
    <title>Long Division with a Non-Zero Remainder</title>
    <statement>
      <p>Use long division to divide <m>37</m> by <m>5</m>. Then express the result using the Division Algorithm.</p>
    </statement>

    <answer>
      <p><me>37 = 7(5) + 2</me></p>
    </answer>

    <solution>
      <p>First, we set up the long division as follows:</p>

      <figure>
        <caption>The 35 goes under the long division symbol and the 5 is written to the left of the symbol.</caption>
        <image source="chapter-5/uneven-long-division-a.png" decorative="yes" width="25%"/>
      </figure>

      <p>Then, we ask ourselves, how many times does <m>5</m> divide into <m>37</m>? It divides 7 times, and we write the <m>7</m> above the one's digit of 37 and above the long division symbol as follows:</p>

      <figure>
        <caption>The 7 is written above the 7 in 37 and above the long division symbol.</caption>
        <image source="chapter-5/uneven-long-division-b.png" decorative="yes" width="25%"/>
      </figure>

      <p>We then multiply <m>7</m> by <m>5</m> to get <m>35</m> and write that below the <m>37</m>.</p>

      <figure>
        <caption>The 35 is written below 37.</caption>
        <image source="chapter-5/uneven-long-division-c.png" decorative="yes" width="25%"/>
      </figure>

      <p>Then we subtract <m>35</m> from <m>37</m> to get <m>2</m>.</p>

      <figure>
        <caption>We put a line under 35 and write 2 below the line.</caption>
        <image source="chapter-5/uneven-long-division.png" decorative="yes" width="25%"/>
      </figure>

      <p>Since <m>2 &lt; 5</m>, the Division Algorithm says we can stop dividing. The number above the long division symbol is the quotient <m>q = 7</m>, and the <m>2</m> we get after the subtraction is the remainder <m>r</m>. Therefore, the Division Algorithm says that <me>37 = 7(5) + 2.</me></p>
    </solution>
  </example>
<example xml:id="long-division-136-by-4">
  <title>Long Division with a Zero Remainder</title>
  <statement>
    <p>Use long division to divide <m>136</m> by <m>4</m>. Then express the result using the Division Algorithm.</p>
  </statement>

  <answer>
    <p><me>136 = 34(4) + 0</me></p>
  </answer>

  <solution>
    <p>First, we set up the long division as follows:</p>

    <figure>
      <caption>The 136 goes under the long division symbol and the 4 is written to the left of the symbol.</caption>
      <image source="chapter-5/even-long-division-b.png" decorative="yes" width="25%"/>
    </figure>

    <p>We ask ourselves, how many times does <m>4</m> divide into the first digit, <m>1</m>? It does not divide evenly, so we consider the first two digits, <m>13</m>. The number <m>4</m> divides into <m>13</m> three times, since <m>3 × 4 = 12</m>.</p>

    <figure>
      <caption>The 3 is written above the 3 in 136 and above the long division symbol.</caption>
      <image source="chapter-5/even-long-division-c.png" decorative="yes" width="25%"/>
    </figure>

    <p>We multiply <m>3 \cdot 4 = 12</m> and write <m>12</m> below <m>13</m>.</p>
        <figure>
      <caption>We write 12 under the hundreds and tens digits, which look like "13".</caption>
      <image source="chapter-5/even-long-division-d.png" decorative="yes" width="25%"/>
    </figure>
        
    <p>Then, we subtract to get <m>1</m>.</p>

    <figure>
      <caption>We put a line under 12 and write 1 below the line.</caption>
      <image source="chapter-5/even-long-division-e.png" decorative="yes" width="25%"/>
    </figure>

    <p>We then bring down the next digit, <m>6</m>, to make <m>16</m>. </p>
    <figure>
      <caption>We bring down the 6 and place it next to the 1.</caption>
      <image source="chapter-5/even-long-division-f.png" decorative="yes" width="25%"/>
    </figure>
        
    <p>The number <m>4</m> divides into <m>16</m> exactly <m>4</m> times, and we write the <m>4</m> above the one's digit in <m>136</m>.</p>

    <figure>
      <caption>The next quotient digit 4 is written above the 6.</caption>
      <image source="chapter-5/even-long-division-g.png" decorative="yes" width="25%"/>
    </figure>

    <p>Since <m>4\cdot 4=16</m>, we write <m>16</m> below the existing <m>16</m>.</p>
<figure>
      <caption>We write 16 below the existing 16 in preparation for another subtraction.</caption>
      <image source="chapter-5/even-long-division-h.png" decorative="yes" width="25%"/>
    </figure>

    <p>We subtract <m>16</m> from <m>16</m> to get <m>0</m>.</p>
    <figure>
      <caption>We write a line below the second <m>16</m>, and write <m>0</m> below the line.</caption>
      <image source="chapter-5/even-long-division.png" decorative="yes" width="25%"/>
    </figure>
    <p>Since <m>r = 0</m>, the division ends here. The number above the long division symbol is the quotient <m>q = 34</m>, and the remainder is <m>r = 0</m>. Therefore, the Division Algorithm says that <me>136 = 34(4) + 0</me>.</p>
  </solution>
</example>
<p>Notice that, in our last example, <me>136 = 34(4) + 0</me> simplifies to <me>136 = 34(4)</me>. We just proved that <m>136</m> factors as <m>34</m> and <m>4</m>. Sound familiar? This is what we want to do with polynomials. Fortunately, a Division Algorithm for polynomials exists as well!</p>

</subsection>
<subsection xml:id="polynomial-division-algorithm">
    
  <title>Polynomial Version</title>
    <p>Before we state the Division Algorithm for Polynomials, we need to define what is the “zero” for polynomials.</p>

<definition xml:id="zero-polynomial">
  <title>The Zero Polynomial</title>
  <statement><p>The <term>zero polynomial</term> is the polynomial whose value is zero for every value of <m>x</m>. We write the zero polynomial as <me>p(x) = 0</me> for all real numbers <m>x</m>.</p></statement>
</definition>

<note>
  <p>Don’t confuse the zero polynomial <m>p(x) = 0</m> with solving a polynomial equation <m>p(x) = 0</m>. While the notations are identical, the contexts are very different. Thankfully, these concepts don’t typically come into direct contact with one another, so the context of the problem will tell you which version of the notation we are using.</p>
</note>


  <theorem xml:id="division-algorithm-polynomials">
    <title>The Division Algorithm</title>
    <statement>
      <p>Let <m>p(x)</m> and <m>d(x)</m> be polynomials, where <m>d(x)</m> is not the zero polynomial. Then there exist unique polynomials, a <term>quotient</term> <m>q(x)</m> and a <term>remainder</term> <m>r(x)</m>, such that</p>
      <p><me>p(x) = q(x) d(x) + r(x)</me></p>
      <p>where the degree of <m>r(x)</m> is less than the degree of <m>d(x)</m>.
    <ul>
        <li>
            <p>
                <m>p(x)</m> is called the <term>dividend</term>.
            </p>
        </li>
        <li>
            <p>
                <m>d(x)</m> is called the <term>divisor</term>.
            </p>
        </li>
    </ul>
    </p>
    </statement>
</theorem>
<example xml:id="polynomial-long-division-x2plus3xminus1-by-xplus4">
  <title>Polynomial Long Division Example</title>
  <statement>
    <p>Use polynomial long division to divide <m>p(x) = x^2 + 3x - 1</m> by <m>d(x) = x + 4</m>. Then express the result using the Division Algorithm for polynomials.</p>
  </statement>

  <answer>
    <p><me>x^2 + 3x - 1 = (x - 1)(x + 4) + 3</me></p>
  </answer>

  <solution>
    <p>First, we set up the division as follows.</p>
    <figure>
      <caption>We set up the long division by putting <m>p(x)</m> under the long division symbol and <m>d(x)</m> to the left of the division symbol</caption>
      <image source="chapter-5/polynomial-long-division-a.png" decorative="yes" width="25%"/>
    </figure>

    <p>We begin by writing a fraction: the numerator is the leading term of <m>p(x)</m> and the denominator is the leading term of <m>d(x)</m>. We then simplify this fraction, and this is the number of times the leading term of the divisor divides the leading term of the dividend.
    In this case, we get the following: <me>\frac{x^2}{x}=x.</me> Since <m>x</m> is a degree 1 term, we will write it above the degree 1 term of the dividend.</p>

    <figure>
      <caption>The leading term <m>x</m> is written above the long division symbol.</caption>
      <image source="chapter-5/polynomial-long-division-b.png" decorative="yes" width="25%"/>
    </figure>

    <p>Next, we multiply the divisor <m>(x + 4)</m> by <m>x</m> to get <m>x^2 + 4x</m>. We write this result below the dividend, make sure the terms with the same powers are vertically lined up. We then write a line under this expression.</p>
       <figure>
      <caption>We write <m>x^2+4x</m> below the <m>x^2</m> and the <m>3x</m> terms.</caption>
      <image source="chapter-5/polynomial-long-division-c.png" decorative="yes" width="25%"/>
    </figure> 
    <p>Next, we subtract <m>x^2 + 4x</m> from the dividend <m>x^2 + 3x - 1</m></p>

    <p>
      <md>
        <mrow>(x^2 + 3x - 1) - (x^2 + 4x) \\</mrow>
        <mrow>= -x - 1</mrow>
      </md>
    </p>

    <p>and write that result below the horizontal line we drew.</p>

    <figure>
      <caption>After subtraction, the new expression is <m>-x - 1</m>.</caption>
      <image source="chapter-5/polynomial-long-division-d.png" decorative="yes" width="25%"/>
    </figure>

    <p>Again, we write a fraction: the numerator is the leading term of <m>-x-1</m> and the denominator is the leading term of <m>d(x)</m>. We then simplify this fraction to get the next division: <me>\frac{-x}{x}=-1.</me> We write the <m>-1</m> above the constant term of the dividend</p>

    <figure>
      <caption><m>-1</m> is written above the constant term in <m>p(x)</m>.</caption>
      <image source="chapter-5/polynomial-long-division-f.png" decorative="yes" width="25%"/>
    </figure>

    <p>and multiply <m>-1</m> by the divisor <m>x+4</m> to get <m>-x-4</m>. We write this product below <m>-x-1</m> and write a line below it.</p>
    <figure>
      <caption>The product <m>-x-4</m> written below <m>-x-1</m>.</caption>
      <image source="chapter-5/polynomial-long-division-g.png" decorative="yes" width="25%"/>
    </figure>

    <p>Now we subtract the two expressions</p>
    
    <p>
      <md>
        <mrow>(-x - 1) - (-x - 4) \\</mrow>
        <mrow>= 3</mrow>
      </md>
    </p>

    <p>and write the 3 below the horizontal line we drew.</p>

    <figure>
      <caption>After the final subtraction, the remainder is <m>3</m>.</caption>
      <image source="chapter-5/polynomial-long-division.png" decorative="yes"  width="25%"/>
    </figure>

    <p>Since the remainder <m>r(x) = 3</m> has degree 0 and the divisor <m>d(x) = x + 4</m> has degree 1, the Division Algorithm tells us we can stop here. The quotient is <m>q(x) = x - 1</m> and the remainder is <m>r(x) = 3</m>. Therefore,</p>

    <p><me>x^2 + 3x - 1 = (x - 1)(x + 4) + 3</me></p>
  </solution>
</example>
<example xml:id="even-polynomial-long-division">
  <title>Polynomial Long Division Example</title>
  <statement>
    <p>Use polynomial long division to divide <m>p(x) = x^4 - x^2 - 2x - 1</m> by <m>d(x) = x^2 - x - 1</m>. Then express the result using the Division Algorithm for polynomials.</p>
  </statement>

  <answer>
    <p><me>x^4 - x^2 - 2x - 1 = (x^2 + x + 1)(x^2 - x - 1) + 0</me></p>
  </answer>

  <solution>
    <p>First, we set up the division as follows.</p>
    <figure>
      <caption>We set up the long division by putting <m>p(x)</m> under the long division symbol and <m>d(x)</m> to the left of the division symbol.</caption>
      <image source="chapter-5/even-poly-division-a.png" decorative="yes" width="40%"/>
    </figure>

    <p>We begin by writing a fraction: the numerator is the leading term of <m>p(x)</m> and the denominator is the leading term of <m>d(x)</m>. We then simplify this fraction; the result tells us how many times the leading term of the divisor divides the leading term of the dividend. In this case,</p>
    <p><me>\frac{x^4}{x^2} = x^2.</me> Since <m>x^2</m> is degree 2, we write it above the degree 2 term of the dividend.</p>

    <figure>
      <caption>The leading quotient term <m>x^2</m> is written above the long division symbol.</caption>
      <image source="chapter-5/even-poly-division-b.png" decorative="yes" width="40%"/>
    </figure>

    <p>Next, we multiply the divisor <m>(x^2 - x - 1)</m> by <m>x^2</m> to get <m>x^4 - x^3 - x^2</m>. We write this result below the dividend, aligning like powers, and draw a horizontal line.</p>
    <figure>
      <caption>We write <m>x^4 - x^3 - x^2</m> below the matching power terms.</caption>
      <image source="chapter-5/even-poly-division-c.png" decorative="yes" width="40%"/>
    </figure>

    <p>Now subtract:</p>
    <p>
      <md>
        <mrow>(x^4 + 0x^3 - x^2 - 2x - 1) - (x^4 - x^3 - x^2) \\</mrow>
        <mrow>= x^3 - 2x - 1</mrow>
      </md>
    </p>

    <figure>
      <caption>After the first subtraction, the new expression is <m>x^3 - 2x - 1</m>.</caption>
      <image source="chapter-5/even-poly-division-d.png" decorative="yes" width="40%"/>
    </figure>

    <p>Again, form the fraction of leading terms and simplify to get the next quotient term:</p>
    <p><me>\frac{x^3}{x^2} = x.</me> We write <m>x</m> in the quotient.</p>

    <figure>
      <caption>The next quotient term <m>x</m> is written above the degree 1 place.</caption>
      <image source="chapter-5/even-poly-division-e.png" decorative="yes" width="40%"/>
    </figure>

    <p>Multiply <m>x</m> by the divisor <m>x^2 - x - 1</m> to get <m>x^3 - x^2 - x</m>. Write this below <m>x^3 - 2x - 1</m> and draw a line.</p>
    <figure>
      <caption>The product <m>x^3 - x^2 - x</m> is written below <m>x^3 - 2x - 1</m>.</caption>
      <image source="chapter-5/even-poly-division-f.png" decorative="yes" width="40%"/>
    </figure>

    <p>Subtract again:</p>
    <p>
      <md>
        <mrow>(x^3 - 2x - 1) - (x^3 - x^2 - x) \\</mrow>
        <mrow>= x^2 - x - 1</mrow>
      </md>
    </p>

    <figure>
      <caption>After the second subtraction, the new expression is <m>x^2 - x - 1</m>.</caption>
      <image source="chapter-5/even-poly-division-g.png" decorative="yes" width="40%"/>
    </figure>

    <p>Form the leading-term fraction once more:</p>
    <p><me>\frac{x^2}{x^2} = 1.</me> We write <m>1</m> in the quotient.</p>

    <figure>
      <caption>The final quotient term <m>1</m> is written above the constant place, completing the quotient <m>x^2 + x + 1</m>.</caption>
      <image source="chapter-5/even-poly-division-h.png" decorative="yes" width="40%"/>
    </figure>

    <p>Multiply <m>1</m> by the divisor to get <m>x^2 - x - 1</m>, write it below, and subtract:</p>
    <p>
      <md>
        <mrow>(x^2 - x - 1) - (x^2 - x - 1) \\</mrow>
        <mrow>= 0</mrow>
      </md>
    </p>

    <figure>
      <caption>After the final subtraction, the remainder is <m>0</m>.</caption>
      <image source="chapter-5/even-poly-division.png" decorative="yes" width="40%"/>
    </figure>

    <p>Since the remainder <m>r(x) = 0</m> has degree less than the divisor <m>d(x) = x^2 - x - 1</m>, the Division Algorithm tells us we can stop here. The quotient is <m>q(x) = x^2 + x + 1</m> and the remainder is <m>r(x) = 0</m>. Therefore,</p>

    <p><me>x^4 - x^2 - 2x - 1 = (x^2 + x + 1)(x^2 - x - 1) + 0</me></p>
  </solution>
</example>
<p>Just like with integers, notice that when the remainder is zero, we get a factorization of the polynomials. Our next goal is to find a consistent way to divide polynomials to get remainders of zero.  But first, we will introduce a simpler way to divide polynomials of certain forms in the next section.</p>
</subsection>

</section>