<section xml:id="synthetic-division">
    <title>Synthetic Division</title>
    <p>Recall that we are looking for a way to factor any polynomial function as <me>p(x)=a_n(x-c_1)(x-c_2)\cdot(x-c_{n-1})(x-c_n)</me>. Since we have seen that there is a relationship between factoring and dividing, notice that all our factors look like <m>x</m> minus a number. So, letâ€™s look at how dividing by <m>x-c</m> and the Division Algorithm work together.</p>

<p>But polynomial long division, as we have seen, can be long, tedious, and cumbersome to write. It turns out that when we divide by <m>x-c</m>, there is a shorthand version of polynomial long division called <term>synthetic division</term> that can make this process faster and less error-prone. Instead of writing a step-by-step method, we will just illustrate how this works in the next three examples.</p>

<example xml:id="synthetic-division-first-example">
  <title>Synthetic Division, First Example</title>

  <statement>
    <p>Use Synthetic Division to divide <m>p(x)=x^3+8x^2+13x+3</m> by <m>d(x)=x+3</m>. Write your final answer using the Division Algorithm.</p>
  </statement>

  <answer>
    <p><me>x^3+8x^2+13x+3=(x^2+5x-2)(x+3)+9</me></p>
  </answer>

  <solution>
    <p>First, we need to write the value of <m>c</m> and box it off. In this case, since <me>x+3=x-(-3)=x-c</me> we have that <m>c=-3</m>. Therefore, we write <m>-3</m> and the box as follows.</p>

    <figure>
      <caption>Write down <m>-3</m> and enclose it on the right and bottom sides.</caption>
      <image source="chapter-5/synthetic-first-example-a.png" decorative="yes" width="50%"/>
    </figure>

    <p>Next, we write the coefficients of <m>p(x)</m> in order from the highest degree term to the lowest degree term. If a degree is missing, use a zero as a placeholder.</p>

    <figure>
      <caption>Write down the coefficients of <m>p(x)=x^3+8x^2+13x+3</m>.</caption>
      <image source="chapter-5/synthetic-first-example-b.png" decorative="yes" width="50%"/>
    </figure>

    <p>Next, leave some space under the coefficients of <m>p(x)</m>. Then, draw a horizontal line under that space.</p>

    <figure>
      <caption>Write a horizontal line under the coefficients, leaving some space between the numbers and the line for additional information.</caption>
      <image source="chapter-5/synthetic-first-example-c.png" decorative="yes" width="50%"/>
    </figure>

    <p>Always bring down the first coefficient and write it below the line.</p>

    <figure>
      <caption>Write the coefficient <m>1</m> below itself under the line.</caption>
      <image source="chapter-5/synthetic-first-example-d.png" decorative="yes" width="50%"/>
    </figure>

    <p>Next, multiply <m>-3</m> by <m>1</m> and write the product <m>-3</m> under the <m>8</m>.</p>

    <figure>
      <caption>Write the product <m>-3</m> below the <m>8</m>.</caption>
      <image source="chapter-5/synthetic-first-example-e.png" decorative="yes" width="50%"/>
    </figure>

    <p>Add <m>8</m> and <m>-3</m> together to get <m>5</m>. Write this number below the <m>-3</m> and under the line.</p>

    <figure>
      <caption>Write the sum <m>5</m> below the line under <m>-3</m>.</caption>
      <image source="chapter-5/synthetic-first-example-f.png" decorative="yes" width="50%"/>
    </figure>

    <p>Next, we multiply <m>-3</m> by <m>5</m> to get <m>-15</m>. We write <m>-15</m> under the <m>13</m>.</p>

    <figure>
      <caption>Write the product <m>-15</m> under <m>13</m>.</caption>
      <image source="chapter-5/synthetic-first-example-g.png" decorative="yes" width="50%"/>
    </figure>

    <p>Then, add <m>13</m> to <m>-15</m> to get <m>-2</m>.</p>

    <figure>
      <caption>Write <m>-2</m> below <m>-15</m> and under the line.</caption>
      <image source="chapter-5/synthetic-first-example-h.png" decorative="yes" width="50%"/>
    </figure>

    <p>Next, multiply <m>-3</m> by <m>-2</m> to get <m>+6</m>. Write <m>6</m> under the <m>3</m>.</p>

    <figure>
      <caption>Write the product <m>6</m> under <m>3</m>.</caption>
      <image source="chapter-5/synthetic-first-example-i.png" decorative="yes" width="50%"/>
    </figure>

    <p>Finally, add <m>3</m> and <m>6</m> together to get <m>9</m>.</p>

    <figure>
      <caption>Write the sum <m>9</m> under the <m>6</m> and below the line.</caption>
      <image source="chapter-5/synthetic-first-example.png" decorative="yes" width="50%"/>
    </figure>

    <p>Now that the synthetic division is done, we have to use the numbers under the line to construct the quotient <m>q(x)</m> and the remainder <m>r(x)</m>.</p>
    <p>The last number in the row is the remainder; so, we have that <m>r(x)=9</m>.</p>
    <p>The remaining three numbers are the coefficients of <m>q(x)</m>. Since <m>p(x)</m> is degree 3 and we divided by a degree 1 polynomial, the quotient <m>q(x)</m> will be a degree 2 polynomial. Therefore, <m>q(x)=x^2+5x-2</m>.</p>

    <p>Using the Division Algorithm, we have that <me>x^3+8x^2+13x+3=(x^2+5x-2)(x+3)+9</me>.</p>
  </solution>
</example>
<example xml:id="synthetic-division-second-example">
  <title>Synthetic Division, Second Example</title>

  <statement>
    <p>Use Synthetic Division to divide <m>p(x)=2x^3-9x^2-5x+36</m> by <m>d(x)=x-4</m>. Write your final answer using the Division Algorithm.</p>
  </statement>

  <answer>
    <p><me>2x^3-9x^2-5x+36=(2x^2-x-9)(x-4)</me></p>
  </answer>

  <solution>
    <p>First, we need to write the value of <m>c</m> and box it off. In this case, since <me>x-4=x-c</me> we have that <m>c=4</m>. Therefore, we write <m>4</m> and the box as follows.</p>

    <figure>
      <caption>Write down <m>4</m> and enclose it on the right and bottom sides.</caption>
      <image source="chapter-5/synthetic-second-example-a.png" decorative="yes" width="50%"/>
    </figure>

    <p>Next, we write the coefficients of <m>p(x)</m> in order from the highest degree term to the lowest degree term. If a degree is missing, use a zero as a placeholder.</p>

    <figure>
      <caption>Write down the coefficients of <m>p(x)=2x^3-9x^2-5x+36</m>.</caption>
      <image source="chapter-5/synthetic-second-example-b.png" decorative="yes" width="50%"/>
    </figure>

    <p>Next, leave some space under the coefficients of <m>p(x)</m>. Then, draw a horizontal line under that space.</p>

    <figure>
      <caption>Write a horizontal line under the coefficients, leaving some space between the numbers and the line for additional information.</caption>
      <image source="chapter-5/synthetic-second-example-c.png" decorative="yes" width="50%"/>
    </figure>

    <p>Always bring down the first coefficient and write it below the line.</p>

    <figure>
      <caption>Write the coefficient <m>2</m> below itself under the line.</caption>
      <image source="chapter-5/synthetic-second-example-d.png" decorative="yes" width="50%"/>
    </figure>

    <p>Next, multiply <m>4</m> by <m>2</m> and write the product <m>8</m> under the <m>-9</m>.</p>

    <figure>
      <caption>Write the product <m>8</m> below the <m>-9</m>.</caption>
      <image source="chapter-5/synthetic-second-example-e.png" decorative="yes" width="50%"/>
    </figure>

    <p>Add <m>-9</m> and <m>8</m> together to get <m>-1</m>. Write this number below the <m>8</m> and under the line.</p>

    <figure>
      <caption>Write the sum <m>-1</m> below the line under <m>8</m>.</caption>
      <image source="chapter-5/synthetic-second-example-f.png" decorative="yes" width="50%"/>
    </figure>

    <p>Next, we multiply <m>4</m> by <m>-1</m> to get <m>-4</m>. We write <m>-4</m> under the <m>-5</m>.</p>

    <figure>
      <caption>Write the product <m>-4</m> under <m>-5</m>.</caption>
      <image source="chapter-5/synthetic-second-example-g.png" decorative="yes" width="50%"/>
    </figure>

    <p>Then, add <m>-5</m> to <m>-4</m> to get <m>-9</m>.</p>

    <figure>
      <caption>Write <m>-9</m> below <m>-4</m> and under the line.</caption>
      <image source="chapter-5/synthetic-second-example-h.png" decorative="yes" width="50%"/>
    </figure>

    <p>Next, multiply <m>4</m> by <m>-9</m> to get <m>-36</m>. Write <m>-36</m> under the <m>36</m>.</p>

    <figure>
      <caption>Write the product <m>-36</m> under <m>36</m>.</caption>
      <image source="chapter-5/synthetic-second-example-i.png" decorative="yes" width="50%"/>
    </figure>

    <p>Finally, add <m>36</m> and <m>-36</m> together to get <m>0</m>.</p>

    <figure>
      <caption>Write the sum <m>0</m> under the <m>-36</m> and below the line.</caption>
      <image source="chapter-5/synthetic-second-example.png" decorative="yes" width="50%"/>
    </figure>

    <p>Now that the synthetic division is done, we have to use the numbers under the line to construct the quotient <m>q(x)</m> and the remainder <m>r(x)</m>.</p>
    <p>The last number in the row is the remainder; so, we have that <m>r(x)=0</m>.</p>
    <p>The remaining three numbers are the coefficients of <m>q(x)</m>. Since <m>p(x)</m> is degree 3 and we divided by a degree 1 polynomial, the quotient <m>q(x)</m> will be a degree 2 polynomial. Therefore, <m>q(x)=2x^2-x-9</m>.</p>

    <p>Using the Division Algorithm, we have that <me>2x^3-9x^2-5x+36=(2x^2-x-9)(x-4)+0=(2x^2-x-9)(x-4)</me>.</p>
  </solution>
</example>
<example xml:id="synthetic-division-third-example">
  <title>Synthetic Division, Third Example</title>

  <statement>
    <p>Use Synthetic Division to divide <m>p(x)=x^4+2x^3+x+2</m> by <m>d(x)=x+2</m>. Write your final answer using the Division Algorithm.</p>
  </statement>

  <answer>
    <p><me>x^4+2x^3+x+2=(x^3+1)(x+2)</me></p>
  </answer>

  <solution>
    <p>First, we need to write the value of <m>c</m> and box it off. In this case, since <me>x+2=x-(-2)</me> we have that <m>c=-2</m>. Therefore, we write <m>-2</m> and the box as follows.</p>

    <figure>
      <caption>Write down <m>-2</m> and enclose it on the right and bottom sides.</caption>
      <image source="chapter-5/synthetic-third-example-a.png" decorative="yes" width="50%"/>
    </figure>

    <p>Next, we write the coefficients of <m>p(x)</m> in order from the highest degree term to the lowest degree term. If a degree is missing, use a zero as a placeholder.</p>

    <figure>
      <caption>Write down the coefficients of <m>p(x)=x^4+2x^3+0x^2+x+2</m>.</caption>
      <image source="chapter-5/synthetic-third-example-b.png" decorative="yes" width="50%"/>
    </figure>

    <p>Next, leave some space under the coefficients of <m>p(x)</m>. Then, draw a horizontal line under that space.</p>

    <figure>
      <caption>Write a horizontal line under the coefficients, leaving some space between the numbers and the line for additional information.</caption>
      <image source="chapter-5/synthetic-third-example-c.png" decorative="yes" width="50%"/>
    </figure>

    <p>Always bring down the first coefficient and write it below the line.</p>

    <figure>
      <caption>Write the coefficient <m>1</m> below itself under the line.</caption>
      <image source="chapter-5/synthetic-third-example-d.png" decorative="yes" width="50%"/>
    </figure>

    <p>Next, multiply <m>-2</m> by <m>1</m> and write the product <m>-2</m> under the <m>2</m>.</p>

    <figure>
      <caption>Write the product <m>-2</m> below the <m>2</m>.</caption>
      <image source="chapter-5/synthetic-third-example-e.png" decorative="yes" width="50%"/>
    </figure>

    <p>Add <m>2</m> and <m>-2</m> together to get <m>0</m>. Write this number below the <m>-2</m> and under the line.</p>

    <figure>
      <caption>Write the sum <m>0</m> below the line under <m>-2</m>.</caption>
      <image source="chapter-5/synthetic-third-example-f.png" decorative="yes" width="50%"/>
    </figure>

    <p>Next, we multiply <m>-2</m> by <m>0</m> to get <m>0</m>. We write <m>0</m> under the <m>0</m> (the next coefficient).</p>

    <figure>
      <caption>Write the product <m>0</m> under <m>0</m>.</caption>
      <image source="chapter-5/synthetic-third-example-g.png" decorative="yes" width="50%"/>
    </figure>

    <p>Then, add <m>0</m> to <m>0</m> to get <m>0</m>.</p>

    <figure>
      <caption>Write <m>0</m> below <m>0</m> and under the line.</caption>
      <image source="chapter-5/synthetic-third-example-h.png" decorative="yes" width="50%"/>
    </figure>

    <p>Next, multiply <m>-2</m> by <m>0</m> to get <m>0</m>. Write <m>0</m> under the <m>1</m>.</p>

    <figure>
      <caption>Write the product <m>0</m> under <m>1</m>.</caption>
      <image source="chapter-5/synthetic-third-example-i.png" decorative="yes" width="50%"/>
    </figure>

    <p>Then, add <m>1</m> and <m>0</m> together to get <m>1</m>.</p>

    <figure>
      <caption>Write the sum <m>1</m> below the line under <m>0</m>.</caption>
      <image source="chapter-5/synthetic-third-example-j.png" decorative="yes" width="50%"/>
    </figure>

    <p>Next, multiply <m>-2</m> by <m>1</m> to get <m>-2</m>. Write <m>-2</m> under the <m>2</m>.</p>

    <figure>
      <caption>Write the product <m>-2</m> under <m>2</m>.</caption>
      <image source="chapter-5/synthetic-third-example-k.png" decorative="yes" width="50%"/>
    </figure>

    <p>Finally, add <m>2</m> and <m>-2</m> together to get <m>0</m>.</p>

    <figure>
      <caption>Write the sum <m>0</m> under the <m>-2</m> and below the line.</caption>
      <image source="chapter-5/synthetic-third-example.png" decorative="yes" width="50%"/>
    </figure>

    <p>Now that the synthetic division is done, we have to use the numbers under the line to construct the quotient <m>q(x)</m> and the remainder <m>r(x)</m>.</p>
    <p>The last number in the row is the remainder; so, we have that <m>r(x)=0</m>.</p>
    <p>The remaining four numbers are the coefficients of <m>q(x)</m>. Since <m>p(x)</m> is degree 4 and we divided by a degree 1 polynomial, the quotient <m>q(x)</m> will be a degree 3 polynomial. Therefore, <me>q(x)=x^3+0x^2+0x+1=x^3+1</me>.</p>

    <p>Using the Division Algorithm, we have that <me>x^4+2x^3+x+2=(x^3+1)(x+2)+0=(x^3+1)(x+2)</me>.</p>
  </solution>
</example>

</section>