<section xml:id="zeroes-and-multiplicity">
    <title>Zeros and Multiplicity</title>
    <subsection xml:id="complete-linear-factorization-of-px">
  <title>The Complete Linear Factorization of <m>p(x)</m></title>

  <p>The ultimate goal of this chapter is to find the complete linear factorization of a polynomial function <m>p(x)</m>.</p>

  <theorem xml:id="complete-linear-factorization-theorem">
    <statement>
      <p>
        The <term>complete linear factorization</term> of a degree <m>n</m> polynomial function <m>p(x)</m> with leading coefficient <m>a_n</m> 
        is given by the formula 
        <me>p(x)=a_n(x-c_1)(x-c_2)\cdots(x-c_{n-1})(x-c_n),</me>
        where <m>c_1</m>, <m>c_2</m>, <m>\ldots</m>, <m>c_{n-1}</m>, <m>c_n</m> 
        are the <m>n</m> (not necessarily distinct) solutions to the equation <m>p(x)=0</m>.
      </p>
    </statement>
  </theorem>

  <p>Let's think about what this statement says.</p>

  <p>
    <ol>
      <li><p>There is a relationship between factoring and solutions to polynomial equations.</p></li>
      <li><p>A degree <m>n</m> polynomial function has <m>n</m> solutions.</p></li>
      <li><p>Since the <m>c_i</m> can be the same value, a solution can be “repeated.”</p></li>
      <li><p>Since this statement is a theorem, there is a proof that this complete linear factorization can always be found.</p></li>
    </ol>
  </p>

  <p>
    While the proof is beyond the scope of this course, our main focus is on the first implication: there is a relationship between factoring and solving equations.
    We already this relationship in Chapter 4: the Zero Product Theorem. 
    We also said in Chapter 4 that the Zero Product Theorem works no matter how many factors there are.
    That means if <me>a_n(x-c_1)(x-c_2)\cdots(x-c_n)=0,</me>
    then finding the solution to the equation <m>p(x)=0</m> is equivalent to solving the <m>n</m> equations
    <me>x-c_1=0\qquad x-c_2=0\qquad\cdots\qquad x-c_n=0.</me>
  </p>

  <p>This is very abstract. So, let's look at a concrete example of this idea in action.</p>

  <example xml:id="using-complete-linear-factorization">
    <title>Using the Complete Linear Factorization to Solve an Equation</title>
    <statement>
      <p>
        The complete linear factorization of the polynomial function 
        <me>p(x)=-2x^4-4x^3+26x^2+28x-48</me> is 
        <me>p(x)=-2(x-3)(x-1)(x+3)(x+4).</me>
        Use the complete linear factorization of the function to solve the equation <m>p(x)=0</m>.
      </p>
    </statement>

    <answer>
      <p>
        <ul>
          <li><p><m>x=-4</m></p></li>
          <li><p><m>x=-3</m></p></li>
          <li><p><m>x=1</m></p></li>
          <li><p><m>x=3</m></p></li>
        </ul>
      </p>
    </answer>

    <solution>
      <p>We will replace the original definition of <m>p(x)</m> with its complete linear factorization and then use the Zero Product Property to solve the equation.</p>

      <p>
        <md>
          <mrow>p(x)\amp=0 \\</mrow>
          <mrow>-2x^4-4x^3+26x^2+28x-48\amp=0 \\</mrow>
          <mrow>-2(x-3)(x-1)(x+3)(x+4)\amp=0 \\</mrow>
          <mrow>(x-3)(x-1)(x+3)(x+4)\amp=0 \\</mrow>
        </md>
    </p><p>
        <md>
          <mrow>x-3\amp=0 \amp x-1\amp=0 \amp x+3\amp=0 \amp x+4\amp=0 \\</mrow>
          <mrow>x\amp=3 \amp x\amp=1 \amp x\amp=-3 \amp x\amp=-4</mrow>
        </md>
      </p>
    </solution>
  </example>
<p>
  It is mysterious, though, how we went from 
  <me>p(x)=-2x^4-4x^3+26x^2+28x-48</me> 
  to 
  <me>p(x)=-2(x-3)(x-1)(x+3)(x+4).</me> 
  None of our factoring techniques show us how to factor this polynomial. 
  Starting in <xref ref="polynomial-long-division"/>, we will develop techniques that will allow us to factor these types of polynomials. 
  But, for the moment, we will explore the relationship between the solutions of <m>p(x)=0</m> 
  and the <m>x</m>-intercepts of the graph of <m>p(x)</m>.
</p>
</subsection>
<subsection xml:id="the-zeroes-of-a-polynomial-function">
  <title>The Zeroes of a Polynomial Function</title>

  <definition xml:id="zero-of-a-polynomial">
    <p>
      A complex number <m>c</m> is a <term>zero</term> of a polynomial function if <m>p(c)=0</m>.
    </p>
  </definition>

  <note xml:id="zeros-alternate-names">
    <p>
      Zeros are also called the <term>roots</term> or <term>solutions</term> of the polynomial equation <m>p(x)=0</m>.
    </p>
  </note>

  <p>
    Wait — a complex number <m>c</m>? You might ask yourself if that is a typo, but that is correct.
    Some of the <m>c_i</m> in our complete linear factorization will be complex!
    Let's look at two examples and see how this plays out.
  </p>

  <example xml:id="finding-zeroes-distinct-real">
    <title>Finding the zeroes of a polynomial function with distinct, real zeroes</title>
    <statement>
      <p>Find the zeroes of the polynomial <m>p(x)=6x^3+9x^2-30x-45.</m></p>
    </statement>

    <answer>
      <p>
        <ul>
          <li><p><m>x=-\frac{3}{2}</m></p></li>
          <li><p><m>x=\sqrt{5}</m></p></li>
          <li><p><m>x=-\sqrt{5}</m></p></li>
        </ul>
      </p>
    </answer>

    <solution>
      <p>
        “Find the zeroes of <m>p(x)=6x^3+9x^2-30x-45</m>” is another way to say “solve the equation <m>6x^3+9x^2-30x-45=0.</m>”
        Therefore, we get the following calculation.
      </p>

      <p>
        <md>
          <mrow>p(x)\amp=0 \\</mrow>
          <mrow>6x^3+9x^2-30x-45\amp=0 \\</mrow>
          <mrow>2x^3+3x^2-10x-15\amp=0 \\</mrow>
          <mrow>(2x^3-10x)+(3x^2-15)\amp=0 \\</mrow>
          <mrow>2x(x^2-5)+3(x^2-5)\amp=0 \\</mrow>
          <mrow>(x^2-5)(2x+3)\amp=0 \\</mrow>
          <mrow>(x-\sqrt{5})(x+\sqrt{5})(2x+3)\amp=0 \\</mrow>
          <mrow>x-\sqrt{5}\amp=0 \amp x+\sqrt{5}\amp=0 \amp 2x+3\amp=0 \\</mrow>
          <mrow>x\amp=\sqrt{5} \amp x\amp=-\sqrt{5} \amp x\amp=-\frac{3}{2}</mrow>
        </md>
      </p>
    </solution>
  </example>

  <p>
    Now, you might note that <m>2x+3=0</m> is not of the form <m>x-c=0</m>, which is required for the complete linear factorization.
    There is a theorem that helps us with that.
  </p>

  <theorem xml:id="rewriting-linear-factors">
    <title>Rewriting Linear Factors that Have Rational Solutions</title>
    <statement>
      <p>Any linear factor of the form <m>(ax-b)</m> can always be rewritten as <m>\left(x-\frac{b}{a}\right)</m>.</p>
    </statement>
  </theorem>

  <p>
    In other words, we could have rewritten <m>(2x+3)</m> as <m>\left(x+\frac{3}{2}\right)</m>,
    but that requires an extra step that is really not necessary when we are solving for <m>x</m>.
  </p>

  <p>Now, let's solve an equation with complex solutions.</p>

  <example xml:id="finding-zeroes-one-real-two-complex">
    <title>Finding the zeroes of a polynomial function with one real solution and two complex solutions</title>
    <statement>
      <p>Find the zeroes of the function <m>p(x)=x^3+27.</m></p>
    </statement>

    <answer>
      <p>
        <ul>
          <li><p><m>x=-3</m></p></li>
          <li><p><m>x=\frac{3}{2}-\frac{3\sqrt{3}}{2}i</m></p></li>
          <li><p><m>x=\frac{3}{2}+\frac{3\sqrt{3}}{2}i</m></p></li>
        </ul>
      </p>
    </answer>

    <solution>
      <p>Since this is a sum of cubes formula, we will first apply that formula.</p>

      <p>
        <md>
          <mrow>p(x)\amp=0 \\</mrow>
          <mrow>x^3+27\amp=0 \\</mrow>
          <mrow>(x+3)(x^2-3x+9)\amp=0</mrow>
        </md>
      </p>

      <p>
        Notice that the factor <m>x^2-3x+9</m> is irreducible since its discriminant is negative.
        But if we allow complex solutions, we can use the quadratic formula to find the complex solutions
        without having to factor <m>x^2-3x+9</m> over the complex numbers.
        The calculation for the quadratic formula is given below.
      </p>

      <p>
        <md>
          <mrow>x\amp=\frac{-b\pm\sqrt{b^2-4ac}}{2a} \\</mrow>
          <mrow>x\amp=\frac{-(-3)\pm\sqrt{(-3)^2-4(1)(9)}}{2(1)} \\</mrow>
          <mrow>x\amp=\frac{3\pm\sqrt{9-36}}{2} \\</mrow>
          <mrow>x\amp=\frac{3\pm\sqrt{-27}}{2} \\</mrow>
          <mrow>x\amp=\frac{3\pm3i\sqrt{3}}{2} \\</mrow>
          <mrow>x\amp=\frac{3}{2}\pm\frac{3\sqrt{3}}{2}i</mrow>
        </md>
      </p>

      <p>Now, we can finish solving the equation.</p>

      <p>
        <md>
          <mrow>(x+3)(x^2-3x+9)\amp=0 \\</mrow>
          <mrow>x+3\amp=0\amp x^2-3x+9\amp=0\\</mrow>
          <mrow>x\amp=-3\amp x\amp=\frac{3}{2}\pm\frac{3\sqrt{3}}{2}i\\</mrow>
        </md>
      </p>
    </solution>
  </example>
<note xml:id="complete-linear-factorization-clarification">
  <p>
    We did not write out the complete linear factorization when solving <xref ref="finding-zeroes-one-real-two-complex"/> since this tends to confuse students at first.
    For the record, the complete linear factorization is 
    <me>(x+3)\left(x-\left(\frac{3}{2}-\frac{3\sqrt{3}}{2}i\right)\right)\left(x-\left(\frac{3}{2}+\frac{3\sqrt{3}}{2}i\right)\right)=0.</me>
    Also, notice that we have see products like <me>\left(x-\left(\frac{3}{2}-\frac{3\sqrt{3}}{2}i\right)\right)\left(x-\left(\frac{3}{2}+\frac{3\sqrt{3}}{2}i\right)\right)</me> before in <xref ref="ex-computing-foil-with-complex-numbers-and-variables"/>.
  </p>
</note>
</subsection>
<subsection xml:id="the-multiplicity-of-a-zero">
  <title>The Multiplicity of a Zero</title>

  <p>
    When we stated 
    <xref ref="complete-linear-factorization-theorem"/>, we mentioned that the solutions to the polynomial equation <m>p(x)=0</m> can be repeated. 
    This leads to the idea of multiplicity, which has two major uses in this chapter:
    <ol>
      <li>
        <p>
          Visualizing how the graph of a polynomial crosses or bounces off the <m>x</m>-axis.
        </p>
      </li>
      <li>
        <p>
          As a trick to simplify solving polynomial inequalities.
        </p>
      </li>
    </ol> 
    We first start by defining multiplicity.
  </p>
  
  <definition xml:id="multiplicity-of-a-zero-definition">
    <title>The Multiplicity of a Zero</title>
    <statement>
      <p>
        Let <m>p(x)</m> be any polynomial function that has a factor of <m>(x-c)^m</m>, where <m>m\geq 1</m>.
        <ul>
          <li>
            <p>
        The exponent <m>m</m> is called the <term>multiplicity</term> of the zero <m>x=c</m>.
            </p>
          </li>
          <li>
            <p>
        If <m>m>1</m>, then <m>x=c</m> is called a <term>repeated zero</term> of <m>p(x)</m>.
            </p>
          </li>
        </ul>
      </p>
    </statement>
  </definition>

  <p>Let's illustrate this definition with an example.</p>

  <example xml:id="finding-multiplicities-of-a-factored-polynomial">
    <title>Finding the Multiplicities of a Factored Polynomial</title>

    <statement>
      <p>Let <m>p(x)=x^3(x-4)^2(x+1)</m>. Find the zeroes and their multiplicities.</p>
    </statement>

    <answer>
      <p>
        <ul>
          <li><p><m>x=0</m> has multiplicity <m>3</m></p></li>
          <li><p><m>x=4</m> has multiplicity <m>2</m></p></li>
          <li><p><m>x=-1</m> has multiplicity <m>1</m></p></li>
        </ul>
      </p>
    </answer>

    <solution>
      <p>
        To find the zeroes, we will set <m>p(x)=0</m> and use the Zero Product Property.
      </p>

      <p>
        <md>
          <mrow>p(x)\amp=0 \\</mrow>
          <mrow>x^3(x-4)^2(x+1)\amp=0 \\</mrow>
          <mrow>x^3\amp=0 \amp (x-4)^2\amp=0 \amp x+1\amp=0 \\</mrow>
          <mrow>\sqrt[3]{x^3}\amp=\sqrt[3]{0} \amp \sqrt{(x-4)^2}\amp=0 \amp x\amp=-1 \\</mrow>
          <mrow>x\amp=0 \amp x-4\amp=0 \amp x\amp=-1 \\</mrow>
          <mrow>x\amp=0 \amp x\amp=4 \amp x\amp=-1</mrow>
        </md>
      </p>

      <p>
        To find the multiplicity of the zeroes, we just have to look back at which factor generated each solution.
      </p>

      <p>
        <ul>
          <li><p>Since <m>x=0</m> came from the factor <m>x^3</m> and  <m>x^3=(x-0)^3</m>, the multiplicity of <m>x=0</m> is <m>3</m>.</p></li>
          <li><p>Since <m>x=4</m> came from the factor <m>(x-4)^2</m>, the multiplicity of <m>x=4</m> is <m>2</m>.</p></li>
          <li><p>Since <m>x=-1</m> came from the factor <m>x+1</m> and <m>x+1=(x+1)^1</m>, the multiplicity of <m>x=-1</m> is <m>1</m>.</p></li>
        </ul>
        Note that both <m>x=0</m> and <m>x=4</m> are repeated zeroes since their multiplicities are greater than 1.
      </p>
    </solution>
  </example>
</subsection>

<subsection xml:id="visualizing-zeroes-as-x-intercepts">
  <title>Visualizing Zeroes as <m>x</m>-intercepts</title>

  <p>
    The real zeroes of a polynomial correspond to the <m>x</m>-intercepts of the graph.
    On top of that, the multiplicity of the zero also dictates the shape of the graph near the <m>x</m>-intercept.
    The key feature is not the exact value of the multiplicity—it is whether the multiplicity is <m>1</m>,
    an odd number greater than <m>1</m>, or an even number.
  </p>

  <theorem xml:id="shape-of-graph-near-x-intercept">
    <title>The Shape of the Graph Near an <m>x</m>-intercept</title>
    <statement>
      <p>
        Suppose <m>x=c</m> is a zero of a polynomial <m>p</m> that has multiplicity <m>m</m>.
        The following figures illustrate the different ways a polynomial can behave near the <m>x</m>-intercept <m>(c,0)</m>.
      </p>

    <figure xml:id="m-equals-1-behavior">
      <caption>The graph will cross as a straight-ish line if <m>m=1</m>.</caption>
      <sidebyside>
        <figure>
          <caption>The graph can either cross from upper left to lower right.</caption>
          <image source="chapter-5/m_1_positive.png" decorative="yes" />
        </figure>

        <figure>
          <caption>Or the graph can cross from lower left to upper right.</caption>
          <image source="chapter-5/m_1_negative.png" decorative="yes"/>
        </figure>
      </sidebyside>
    </figure>

    <figure xml:id="m-odd-greater-than-1-behavior">
      <caption>The graph will cross at <m>(c,0)</m> similar to how <m>y=x^m</m> crosses at <m>(0,0)</m> if <m>m&gt;1</m> and is odd.</caption>
      <sidebyside>
        <figure>
          <caption>
            The graph can either cross from upper left to lower right while flattening at <m>(c,0)</m>.
          </caption>
          <image source="chapter-5/m_odd_positive.png" decorative="yes"/>
        </figure>

        <figure>
          <caption>
            Or the graph can cross from lower left to upper right while flattening at <m>(c,0)</m>.
          </caption>
          <image source="chapter-5/m_odd_negative.png" decorative="yes"/>
        </figure>
      </sidebyside>
    </figure>

    <figure xml:id="m-even-behavior">
      <caption>The graph will bounce off the <m>x</m>-axis at <m>(c,0)</m> if <m>m</m> is even.</caption>
      <sidebyside>
        <figure>
          <caption>Bounce off the <m>x</m>-axis at <m>(c,0)</m> from above.</caption>
          <image source="chapter-5/m_even_above.png" decorative="yes"/>
        </figure>

        <figure>
          <caption>Bounce off the <m>x</m>-axis at <m>(c,0)</m> from below.</caption>
          <image source="chapter-5/m_even_below.png" decorative="yes"/>
        </figure>
      </sidebyside>
    </figure>

    </statement>
  </theorem>
  <example xml:id="determine-cross-or-bounce-at-x-intercept">
  <title>Determine if the Graph Will Cross or Bounce at an <m>x</m>-intercept</title>

  <statement>
    <p>
      Let <m>p(x)=-2(x-3)^2(x+4)</m>. 
      Find the zeroes, their multiplicities, and classify whether the graph will cross or bounce at the zeroes.
    </p>
  </statement>

  <solution>
    <p>
      <ul>
        <li>
          <p>
            There is a zero at <m>x=3</m> with even multiplicity. 
            The graph will bounce off the <m>x</m>-axis at <m>(3,0)</m>.
          </p>
        </li>
        <li>
          <p>
            There is a zero at <m>x=-4</m> with odd multiplicity. 
            The graph will cross the <m>x</m>-axis at <m>(-4,0)</m>.
          </p>
        </li>
      </ul>
    </p>
  </solution>
</example>

</subsection>

</section>