<section xml:id="vertex-form-of-a-quadratic-function">
  <title>The Vertex Form of a Quadratic Function</title>

  <subsection xml:id="writing-quadratic-equations-in-vertex-form">
    <title>Writing Quadratic Equations in Vertex Form</title>

    <definition xml:id="standard-form-of-a-quadratic">
      <title>The Standard Form of a Quadratic</title>
      <statement>
        <p>The <term>standard form</term> of a quadratic function is
        <me>f(x) = ax^2 + bx + c.</me></p>
      </statement>
    </definition>
    <p>
      The standard form of a quadratic function is not very useful since the majority of its features,
      like its vertex and axis of symmetry, are not baked into the algebraic expression
      <m>ax^2 + bx + c</m>. So, while the standard form is useful for solving equations in one variable,
      it is not as useful when set equal to <m>y</m> instead of 0.
      Using the theory of transformations from Chapter 7, mathematicians discovered that the
      vertex form of the function is the correct way to encapsulate all the important information
      of the graph.
    </p>

    <theorem xml:id="vertex-form-and-related-information">
      <title>The Vertex Form and Related Information</title>

      <statement>
        <p>Let <m>f(x) = ax^2 + bx + c</m> be a quadratic function in standard form.
        The <term>vertex form</term> of a quadratic function is given by
        <me>f(x) = a(x - h)^2 + k,</me>
        where <m>h</m> and <m>k</m> are the coordinates for the vertex of the function.</p>

      <p>There are two important definitions related to the vertex form.

      <ul>
        <li>
          The <term>vertex</term> of the parabola is the absolute minimum (when <m>a &gt; 0</m>)
          or the absolute maximum (when <m>a &lt; 0</m>) of the function.
          Note that the vertex is both a local and absolute extremum.
        </li>

        <li>
          The <term>axis of symmetry</term> of a parabola is the vertical line that divides the parabola
          into two mirror images. Every point on one side of this line has a corresponding point
          on the other side that is the same distance from the line.
        </li>
      </ul>
    </p>
      <figure xml:id="parabola-axis-of-symmetry">
        <caption>
          The graph of a generic parabola with the vertex and axis of symmetry labeled.
          Two mirrored points are labeled, and the distances from the points to the axis
          of symmetry are shown as equal.
        </caption>

        <sidebyside>

          <figure>
            <caption>An upwards-facing parabola.</caption>
            <image source="chapter-4-14/labeled-upwards-parabola.png" width="40%">
              <shortdescription>A labeled, upwards-facing parabola.</shortdescription>
            </image>
          </figure>

          <figure>
            <caption>A downwards-facing parabola.</caption>
            <image source="chapter-4-14/labeled-downwards-parabola.png" width="40%">
              <shortdescription>A labeled, downwards-facing parabola.</shortdescription>
            </image>
          </figure>

        </sidebyside>
      </figure>

      </statement>
    </theorem>

    <p>
      There are two methods for finding the vertex form from the standard form.
      The first one uses completing the square to accomplish the transformation.
    </p>

    <example xml:id="completing-the-square-to-vertex-form">
      <title>Using Completing the Square to Convert from Standard to Vertex Form</title>

      <statement>
        <p>Convert <m>f(x) = 3x^2 - 12x + 13</m> to vertex form.</p>
      </statement>
      <answer>
        <p>
          <m>f(x)= 3(x - 2)^2 + 1</m>
        </p>
      </answer>
      <solution><p>
<md>
  <mrow>f(x)\amp= 3x^2 - 12x + 13 \\</mrow>
  <mrow>f(x) - 13\amp= 3x^2 - 12x \\</mrow>
  <mrow>\frac{f(x)}{3} - \frac{13}{3}\amp= \frac{3x^2}{3} - \frac{12}{3}x \\</mrow>
  <mrow>\frac{f(x)}{3} - \frac{13}{3}\amp= x^2 - 4x \\</mrow>
  <mrow>\frac{f(x)}{3} - \frac{13}{3}\amp= x^2 - 4x \amp \frac{-4}{2}\amp= -2 \amp (-2)^2\amp= 4 \\</mrow>
  <mrow>\frac{f(x)}{3} - \frac{13}{3} + 4\amp= x^2 - 4x + 4 \\</mrow>
  <mrow>\frac{f(x)}{3} - \frac{13}{3} + 4\amp= (x - 2)^2 \\</mrow>
  <mrow>3\left(\frac{f(x)}{3}\right) - 3\left(\frac{13}{3}\right) + 3(4)\amp= 3(x - 2)^2 \\</mrow>
  <mrow>f(x) - 13 + 12\amp= 3(x - 2)^2 \\</mrow>
  <mrow>f(x) - 1\amp= 3(x - 2)^2 \\</mrow>
  <mrow>f(x)\amp= 3(x - 2)^2 + 1</mrow>
</md>
</p>
      </solution>
    </example>
<p>While completing the square gets the job done, it is very cumbersome and time-consuming to do. It would be nice to have a formula for the <m>h</m> and <m>k</m> in the vertex formula. If we complete the square on <m>f(x)=ax^2+bx+c</m>, we get</p>

<p>
  <me>f(x)=a\left(x+\frac{b}{2a}\right)^2+c-\frac{b^2}{4a}</me>
</p>

<p>This tells us that</p>

<p>
  <md>
    <mrow>h\amp=-\frac{b}{2a} \amp k\amp=c-\frac{b^2}{4a}</mrow>
  </md>
</p>

<p>But, notice what happens when we evaluate <m>f\left(-\frac{b}{2a}\right)</m></p>

<p>
  <md>
    <mrow>f\left(-\frac{b}{2a}\right)\amp=a\left(-\frac{b}{2a}+\frac{b}{2a}\right)^2+c-\frac{b^2}{4a} \\</mrow>
    <mrow>\amp=a(0)^2+k \\</mrow>
    <mrow>\amp=k</mrow>
  </md>
</p>

<p>Therefore, the pair of formula you should use and memorize is</p>

<p>
  <md>
    <mrow>h\amp=-\frac{b}{2a} \amp k\amp=f\left(-\frac{b}{2a}\right)</mrow>
  </md>
</p>

<theorem xml:id="formula-for-the-vertex-of-a-parabola">
  <title>Formula for the Vertex of a Parabola</title>
  <statement>
    <p>Let <m>f(x)=ax^2+bx+c</m> be a quadratic function. Then the formula for the vertex is</p>
    <p>
      <me>(h,k)=\left(-\frac{b}{2a},f\left(-\frac{b}{2a}\right)\right)</me>
    </p>
    <p>We can also rewrite this as the pair of equations <md><mrow>h\amp=-\frac{b}{2a}\amp k\amp=f\left(\frac{-b}{2a}\right)</mrow></md></p>
  </statement>
</theorem>

<p>While these formulas still look unwieldy in this form, in practice they are very easy to use.</p>

<example xml:id="using-formula-for-h-and-k">
  <title>Using the Formula for <m>h</m> and <m>k</m> to find the Vertex Form of a Quadratic Function</title>
  <statement>
    <p>Write <m>f(x)=2x^2-4x-6</m> in vertex form.</p>
  </statement>
  <answer>
    <p><m>f(x)=2(x-1)^2-8</m></p>
  </answer>
  <solution>
    <p>Since <m>a=2</m> and <m>b=-4</m>, we have that</p>
    <p>
      <me>h=-\frac{b}{2a}=-\frac{-4}{2(2)}=1.</me>
    </p>
    <p>Then, evaluate <m>f(1)</m> to find the value of <m>k</m>:</p>
    <p>
      <md>
        <mrow>f(x)\amp=2x^2-4x-6 \\</mrow>
        <mrow>f(1)\amp=2(1)^2-4(1)-6 \\</mrow>
        <mrow>f(1)\amp=2-4-6 \\</mrow>
        <mrow>f(1)\amp=-8</mrow>
      </md>
    </p>
    <p>Therefore, the vertex form is</p>
    <p>
      <me>f(x)=2(x-1)^2-8.</me>
    </p>
  </solution>
</example>
</subsection>
<subsection xml:id="graphing-quadratic-functions-using-the-vertex-form">
  <title>Graphing Quadratic Functions Using the Vertex Form</title>

  <p>The vertex form gives us enough information to easily graph any quadratic function.</p>

  <lemma xml:id="graphing-quadratic-functions">
    <title>Graphing Quadratic Functions</title>
    <statement>
      <p>Let <m>f(x) = a(x - h)^2 + k</m> be a quadratic function in vertex form. Perform the following steps to plot its graph.</p>

      <p>
        <ol>
          <li><p>Plot the vertex <m>(h, k)</m>.</p></li>
          <li><p>To find another point, add <m>1</m> to <m>h</m> and add <m>a \cdot 1^2</m> to <m>k</m>. Then plot the point.</p></li>
          <li><p>To find an additional point, add <m>2</m> to <m>h</m> and add <m>a \cdot 2^2</m> to <m>k</m>. Then plot the point.</p></li>
          <li><p>Use the axis of symmetry to find and plot the last two points.</p></li>
          <li><p>Draw a parabola through all five points.</p></li>
        </ol>
      </p>
    </statement>
  </lemma>
  <example xml:id="how-to-graph-a-quadratic-function-a-greater-0">
  <title>How to Graph a Quadratic Function, <m>a &gt; 0</m></title>

  <statement>
    <p>Graph the function <m>f(x) = 2x^2 - 4x + 5</m>.</p>
  </statement>

  <answer>
    <figure>
      <caption>The graph of <m>f(x) = 2x^2 - 4x + 5</m> with vertex <m>(1, -3)</m> and axis of symmetry <m>x = 1</m>.</caption>
      <image source="chapter-4-14/example-upwards-parabola-final.png" decorative="yes" width="60%"></image>
    </figure>
  </answer>

  <solution>
    <p>First, we note that <m>a = 2</m> and <m>b = -4</m>. Using the formula for <m>h</m>, we get:</p>

    <p>
      <md>
        <mrow>h \amp= -\frac{b}{2a} \\</mrow>
        <mrow>\amp= -\frac{-4}{2(2)} \\</mrow>
        <mrow>\amp= \frac{4}{4} \\</mrow>
        <mrow>\amp= 1</mrow>
      </md>
    </p>

    <p>Next, we compute the value of <m>k</m>:</p>

    <p>
      <md>
        <mrow>k \amp= f(1) \\</mrow>
        <mrow>\amp= 2(1)^2 - 4(1) + 5 \\</mrow>
        <mrow>\amp= 2 - 4 + 5 \\</mrow>
        <mrow>\amp= 3</mrow>
      </md>
    </p>

    <p>Therefore, we know the vertex is <m>(1, 3)</m> and the axis of symmetry is the vertical line <m>x = 1</m>. We start the graph by plotting the vertex and axis of symmetry.</p>

    <figure>
      <caption>The graph of <m>(1, 3)</m> and <m>x = 1</m>.</caption>
      <image source="chapter-4-14/example-upwards-parabola-1.png" decorative="yes" width="60%">
      </image>
    </figure>

    <p>Next, we compute two additional points. The first point is:</p>

    <p>
      <md>
        <mrow>\text{first additional point } \amp= (h + 1, k + a(1)^2) \\</mrow>
        <mrow>\amp= (1 + 1, 3 + 2(1)^2) \\</mrow>
        <mrow>\amp= (2, 5)</mrow>
      </md>
    </p>

    <p>and the second point is:</p>

    <p>
      <md>
        <mrow>\text{second additional point } \amp= (h + 2, k + a(2)^2) \\</mrow>
        <mrow>\amp= (1 + 2, 3 + 2(2)^2) \\</mrow>
        <mrow>\amp= (3, 11)</mrow>
      </md>
    </p>

    <p>We plot these two points as well.</p>

    <figure>
      <caption>The points <m>(2, 5)</m> and <m>(3, 11)</m> are added to the previous graph.</caption>
      <image source="chapter-4-14/example-upwards-parabola-2.png" decorative="yes" width="60%">
      </image>
    </figure>

    <p>Next, we find the two mirrored points. They will have the same <m>y</m>-coordinates as <m>(2, 5)</m> and <m>(3, 11)</m>, but the <m>x</m>-coordinates will be <m>h - 1</m> and <m>h - 2</m>, respectively. Therefore, the mirrored points are <m>(0,5)</m> and <m>(-1, 11)</m>. We plot these additional points.</p>

    <figure>
      <caption>The points <m>(0,5)</m> and <m>(-1, 11)</m> are added to the previous graph.</caption>
      <image source="chapter-4-14/example-upwards-parabola-3.png" decorative="yes" width="60%"/>
    </figure>

    <p>Finally, we connect all the points with a parabola to get the final graph.</p>

    <figure>
      <caption>The graph of <m>f(x) = 2x^2 - 4x + 5</m> with vertex <m>(1, 3)</m> and axis of symmetry <m>x = 1</m>.</caption>
      <image source="chapter-4-14/example-upwards-parabola-final.png" decorative="yes" width="60%">
      </image>
    </figure>
  </solution>
</example>
<example xml:id="how-to-graph-a-quadratic-function-a-less-0">
  <title>How to Graph a Quadratic Function, <m>a &lt; 0</m></title>

  <statement>
    <p>Graph the function <m>f(x) = -3x^2 - 12x - 8</m>.</p>
  </statement>

  <answer>
    <figure>
      <caption>The graph of <m>f(x) = -3x^2 - 12x - 8</m> with vertex <m>(-2, 4)</m> and axis of symmetry <m>x = -2</m>.</caption>
      <image source="chapter-4-14/example-downwards-parabola-final.png" decorative="yes" width="60%"/>
    </figure>
  </answer>

  <solution>
    <p>First, identify the coefficients <m>a = -3</m> and <m>b = -12</m>. Using the formula for <m>h</m>, we get:</p>

    <p>
      <md>
        <mrow>h \amp= -\frac{b}{2a} \\</mrow>
        <mrow>\amp= -\frac{-12}{2(-3)} \\</mrow>
        <mrow>\amp= \frac{12}{-6} \\</mrow>
        <mrow>\amp= -2</mrow>
      </md>
    </p>

    <p>Next, compute <m>k</m>:</p>

    <p>
      <md>
        <mrow>k \amp= f(-2) \\</mrow>
        <mrow>\amp= -3(-2)^2 - 12(-2) - 8 \\</mrow>
        <mrow>\amp= -12 + 24 - 8 \\</mrow>
        <mrow>\amp= 4</mrow>
      </md>
    </p>

    <p>The vertex is <m>(-2, 4)</m> and the axis of symmetry is the vertical line <m>x = -2</m>. Begin the graph by plotting the vertex and axis of symmetry.</p>

    <figure>
      <caption>The vertex <m>(-2, 4)</m> and axis <m>x = -2</m> are plotted.</caption>
      <image source="chapter-4-14/example-downwards-parabola-1.png" decorative="yes" width="60%"/>
    </figure>

    <p>Now compute two additional points one and two units to the right of the vertex:</p>

    <p>
      <md>
        <mrow>(h + 1, k + a(1)^2) \amp= (-2 + 1, 4 + (-3)(1)^2) \\</mrow>
        <mrow>\amp= (-1, 1)</mrow>
      </md>
    </p>

    <p>
      <md>
        <mrow>(h + 2, k + a(2)^2) \amp= (-2 + 2, 4 + (-3)(2)^2) \\</mrow>
        <mrow>\amp= (0, -8)</mrow>
      </md>
    </p>

    <p>Plot these two points.</p>

    <figure>
      <caption>The points <m>(-1, 1)</m> and <m>(0, -8)</m> are added.</caption>
      <image source="chapter-4-14/example-downwards-parabola-2.png" decorative="yes" width="60%"/>
    </figure>

    <p>Reflect across the axis <m>x = -2</m> to obtain the mirrored points:</p>

    <p>
      <md>
        <mrow>(h - 1, 1) \amp= (-3, 1) \\</mrow>
        <mrow>(h - 2, -8) \amp= (-4, -8)</mrow>
      </md>
    </p>

    <p>Plot these mirrored points as well.</p>

    <figure>
      <caption>The reflected points <m>(-3, 1)</m> and <m>(-4, -8)</m> are added.</caption>
      <image source="chapter-4-14/example-downwards-parabola-3.png" decorative="yes" width="60%"/>
    </figure>

    <p>Finally, connect the points with a smooth downward-opening parabola to obtain the final graph.</p>

    <figure>
      <caption>The graph of <m>f(x) = -3x^2 - 12x - 8</m> with vertex <m>(-2, 4)</m> and axis of symmetry <m>x = -2</m>.</caption>
      <image source="chapter-4-14/example-downwards-parabola-final.png" decorative="yes" width="60%"/>
    </figure>
  </solution>
</example>

</subsection>
<subsection xml:id="graphing-quadratic-functions-using-intercepts">
  <title>Graphing Quadratic Functions Using Intercepts</title>

  <p>While the previous method always works, it requires you to remember some unusual formulas. When the parabola crosses the <m>x</m>-axis, you can instead use the vertex, the <m>y</m>-intercept, and the <m>x</m>-intercepts to plot key points. The next example shows how to do this.</p>

  <example xml:id="graphing-using-intercepts">
    <title>How to Graph a Quadratic Function Using Intercepts</title>

    <statement>
      <p>Graph the function <m>f(x) = -2x^2 - 8x - 6.</m></p>
    </statement>

    <answer>
      <figure>
        <caption>The graph of <m>f(x) = -2x^2 - 8x - 6</m>, the vertex <m>(-2, 2)</m>, and the intercepts <m>(-3, 0)</m>, <m>(-1, 0)</m>, and <m>(0, -6)</m>.</caption>
        <image source="chapter-4-14/example-quadratic-parabola-intercepts-final.png" width="60%" decorative="yes"/>
      </figure>
    </answer>

    <solution>
      <p>Since <m>a = -2</m> and <m>b = -8</m>, we use the formulas for <m>h</m> and <m>k</m> to find the vertex.</p>

      <p>
        <md>
          <mrow>h \amp= -\frac{b}{2a} \\</mrow>
          <mrow>\amp= -\frac{-8}{2(-2)} \\</mrow>
          <mrow>\amp= -\frac{8}{4} \\</mrow>
          <mrow>h \amp= -2</mrow>
        </md>
      </p>

      <p>
        <md>
          <mrow>k \amp= f(-2) \\</mrow>
          <mrow>\amp= -2(-2)^2 - 8(-2) - 6 \\</mrow>
          <mrow>\amp= -8 + 16 - 6 \\</mrow>
          <mrow>k \amp= 2</mrow>
        </md>
      </p>

      <p>Therefore, the vertex is <m>(-2, 2)</m>. To find the <m>x</m>-intercepts, we use the quadratic formula:</p>

      <p>
        <md>
          <mrow>x \amp= \frac{-b \pm \sqrt{b^2 - 4ac}}{2a} \\</mrow>
          <mrow>\amp= \frac{-(-8) \pm \sqrt{(-8)^2 - 4(-2)(-6)}}{2(-2)} \\</mrow>
          <mrow>\amp= \frac{8 \pm \sqrt{64 - 48}}{-4} \\</mrow>
          <mrow>\amp= \frac{8 \pm \sqrt{16}}{-4}</mrow>
        </md>
      </p>

      <p>
        <md>
          <mrow>x \amp= \frac{8 - 4}{-4} \amp x \amp= \frac{8 + 4}{-4} \\</mrow>
          <mrow>x \amp= \frac{4}{-4} \amp x \amp= \frac{12}{-4} \\</mrow>
          <mrow>x \amp= -1 \amp x \amp= -3</mrow>
        </md>
      </p>

      <p>Therefore, the <m>x</m>-intercepts are <m>(-1, 0)</m> and <m>(-3, 0)</m>. To find the <m>y</m>-intercept, we evaluate <m>f(0)</m>:</p>

      <p><me>f(0) = -2(0)^2 - 8(0) - 6 = -6</me></p>

      <p>Therefore, the <m>y</m>-intercept is <m>(0, -6)</m>. We then plot all four points and sketch the parabola through them to obtain the graph.</p>

      <figure>
        <caption>The graph of <m>f(x) = -2x^2 - 8x - 6</m>, showing the vertex <m>(-2, 2)</m> and intercepts <m>(-3, 0)</m>, <m>(-1, 0)</m>, and <m>(0, -6)</m>.</caption>
        <sidebyside>
          <figure>
            <caption>A plot showing the vertex and intercepts before drawing the parabola.</caption>
            <image source="chapter-4-14/example-quadratic-parabola-intercepts-1.png" decorative="yes" width="60%"/>
          </figure>
          <figure>
            <caption>The completed parabola passing through all four points.</caption>
            <image source="chapter-4-14/example-quadratic-parabola-intercepts-final.png" decorative="yes" width="60%"/>
          </figure>
        </sidebyside>
      </figure>
    </solution>
  </example>
</subsection>

</section>
