<section xml:id="sec-the-zero-product-property">
    <title>The Zero Product Property</title>

    <subsection xml:id="subsec-quadratic-equations">
        <title>Quadratic Equations</title>

        <definition xml:id="def-quadratic-equations">
            <title>Quadratic Equations</title>
            <statement>
                <p>
                    Let <m>a</m>, <m>b</m>, and <m>c</m> be real numbers with <m>a \ne 0</m>.
                    Any equation of the form <me>ax^2 + bx + c = 0</me> is called a <term>quadratic equation</term> in <m>x</m>.
                </p>
            </statement>
        </definition>

        <example xml:id="ex-determine-if-an-equation-is-quadratic">
            <title>Determine if an Equation is Quadratic</title>
            <statement>
                <p>
                    Which of the following equations are examples of a quadratic equation?
                </p>
                <p>
                    <ul>
                        <li><p><m>3x^2 + 4x - 9 = 0</m></p></li>
                        <li><p><m>3(x - 2)^2 = 1</m></p></li>
                        <li><p><m>5\sqrt{x - 1} + x = 0</m></p></li>
                        <li><p><m>\frac{1}{x} + x^2 - 4 = 0</m></p></li>
                    </ul>
                </p>
            </statement>
            <solution>
                <p>
                    <ul>
                        <li><p>This is a quadratic equation with <m>a=3</m>, <m>b=4</m>, and <m>c=-9</m>.</p></li>
                        <li><p>If we fully simplify this equation, we get:
                            <md>
                        <mrow>3(x - 2)^2 \amp= 1</mrow>
                        <mrow>3(x^2 - 4x + 4) - 1 \amp= 0</mrow>
                        <mrow>3x^2 - 12x + 12 - 1 \amp= 0</mrow>
                        <mrow>3x^2 - 12x + 11 \amp= 0</mrow>
                            </md>
                        </p>
                        </li>
                        <li><p>Since the variable is under the square root, this equation cannot be quadratic.</p></li>
                        <li><p>Since we have a variable in the denominator, this equation cannot be quadratic.</p></li>
                    </ul>
                </p>
            </solution>
        </example>
    </subsection>

    <subsection xml:id="subsec-the-zero-product-property">
        <title>The Zero Product Property</title>
        <p>
            Factoring is the most important tool we have to solve equations and to understand the properties of polynomial and rational functions.
            Factoring gets a lot of its power from the Zero Product Property.
            This property allows us to split a factored equation into two or more simpler equations that are easier to solve than the original equation,
            but we have to satisfy one condition: the factorization must be equal to zero.
        </p>

        <theorem xml:id="def-zero-product-property">
            <title>The Zero Product Property</title>
            <statement>
                <p>
                    Let <m>A</m> and <m>B</m> be algebraic expressions such that <m>AB = 0</m>.
                    Then <m>A = 0</m> or <m>B = 0</m>.
                </p>
            </statement>
        </theorem>

        <p>
            One of the most common issues that occurs is when people try to apply this equation when the non-factored side is nonzero.
            Let's see what happens in this case when we inappropriately apply this property to the equation <me>(x + 3)(x - 4) = 2</me>.
        </p>

        <p>
            <md>
                <mrow>x + 3 \amp= 2 \amp x - 4 \amp= 2</mrow>
                <mrow>x \amp= -1 \amp x \amp= 6</mrow>
            </md>
        </p>

        <p>
            Now, let's check our work.
        </p>

        <p>
            <md>
                <mrow>(x + 3)(x - 4) \amp= 2 \amp (x + 3)(x - 4) \amp= 2</mrow>
                <mrow>(2 + 3)(2 - 4) \amp= 2 \amp (6 + 3)(6 - 4) \amp= 2</mrow>
                <mrow>5(-2) \amp\ne 2 \amp (9)(2) \amp\ne 2</mrow>
            </md>
        </p>

        <p>
            Notice that both values of <m>x</m> fail the check, which means that neither of them were a solution.
            By making one side of the equation equal to zero, we are guaranteeing that this process will always result in solutions.
        </p>
    </subsection>

    <subsection xml:id="subsec-solving-equations-by-factoring">
        <title>Solving Equations by Factoring</title>

        <example xml:id="ex-solve-by-factoring-a-gcf">
            <title>Solve by Factoring a GCF</title>
            <statement>
                <p>
                    Solve the equation <m>4x^2 - 2x = 0</m>.
                </p>
            </statement>
            <answer>
                <p>
                    <ul>
                        <li><p><m>x = 0</m></p></li>
                        <li><p><m>x = \frac{1}{2}</m></p></li>
                    </ul>
                </p>
            </answer>
            <solution>
                <p>
                    To solve this problem, we will factor out a GCF which creates a product equal to zero.
                    Then we apply the Zero Product Property.
                    The following calculation shows us all the steps we need to perform.
                </p>
                <p>
                    <md>
                        <mrow>4x^2 - 2x \amp= 0</mrow>
                        <mrow>2x(2x - 1) \amp= 0</mrow>
                        <mrow>2x \amp= 0 \amp 2x - 1 \amp= 0</mrow>
                        <mrow>x \amp= 0 \amp 2x \amp= 1</mrow>
                        <mrow>\amp \amp x \amp= \frac{1}{2}</mrow>
                    </md>
                </p>
                <p>
                    Therefore, the solutions are <m>x = 0</m> and <m>x = \frac{1}{2}</m>.
                </p>
            </solution>
        </example>

        <example xml:id="ex-solve-using-the-zero-product-property">
            <title>Solve using the Zero Product Property</title>
            <statement>
                <p>
                    Solve the equation <m>(3x - 2)(x + 4) = 0</m>.
                </p>
            </statement>
            <answer>
                <p>
                    <ul>
                        <li><p><m>x = \frac{3}{2}</m></p></li>
                        <li><p><m>x = -4</m></p></li>
                    </ul>
                </p>
            </answer>
            <solution>
                <p>
                    This problem is already factored.
                    All we have to do is apply the Zero Product Property and solve for <m>x</m>.
                    The following calculation shows us the necessary steps.
                </p>
                <p>
                    <md>
                        <mrow>(3x - 2)(x + 4) \amp= 0</mrow>
                        <mrow>3x - 2 \amp= 0 \amp x + 4 \amp= 0</mrow>
                        <mrow>3x \amp= 2 \amp x \amp= -4</mrow>
                        <mrow>x \amp= \frac{3}{2} \amp x \amp= -4</mrow>
                    </md>
                </p>
                <p>
                    Therefore, the solutions are <m>x = \frac{3}{2}</m> and <m>x = -4</m>.
                </p>
            </solution>
        </example>

        <example xml:id="ex-solving-using-the-zero-product-property-on-three-factors">
            <title>Solving Using the Zero Product Property on 3 or More Factors</title>
            <statement>
                <p>
                    Solve the equation <m>(x - 2)(x + 3)(x - 1) = 0</m>.
                </p>
            </statement>
            <answer>
                <p>
                    <ul>
                        <li><p><m>x = 2</m></p></li>
                        <li><p><m>x = -3</m></p></li>
                        <li><p><m>x = 1</m></p></li>
                    </ul>
                </p>
            </answer>
            <solution>
                <p>
                    Due to the Associative Property of Multiplication, we can extend the Zero Product Property to any number of factors
                    as long as the overall product is equal to zero.
                    The following calculation demonstrates how to do this for this equation.
                </p>
                <p>
                    <md>
                        <mrow>(x - 2)(x + 3)(x - 1) \amp= 0</mrow>
                        <mrow>x - 2 \amp= 0 \amp x + 3 \amp= 0 \amp x - 1 \amp= 0</mrow>
                        <mrow>x \amp= 2 \amp x \amp= -3 \amp x \amp= 1</mrow>
                    </md>
                </p>
                <p>
                    Therefore, the solutions are <m>x = 2</m>, <m>x = -3</m>, and <m>x = 1</m>.
                </p>
            </solution>
        </example>
    </subsection>
</section>
